\begin{equation}
\boldsymbol{\alpha_t(i)} = P(\obsseq{1}{2}{t}, q_t = S_i \given \lambda)
\hspace{9.8em}\label{eq:fw:forw}
\end{equation}

\begin{align}
\alpha_1(i) = \pi_i b_i(O_1),\qquad &1 \leq i \leq N.
\label{eq:fw:forw:init} \\
\alpha_{t+1}(j) = [\sum_{i=1}^N \alpha_t(i) a_{ij}] b_j(O_{t+1}),
\qquad &1 \leq t \leq T - 1, \nonumber \\
&1 \leq j \leq N.\label{eq:fw:forw:loop}
\end{align}

\begin{equation}
\boldsymbol{\beta_t(i)} = P(\obsseq{t+1}{t+2}{T} \given q_t = S_i, \lambda)
\hspace{8em}\label{eq:fw:back}
\end{equation}

\begin{align}
\beta_T(i) = 1,\qquad &1 \leq i \leq N.
\label{eq:fw:back:init} \\
\beta_{t}(i) = \sum_{j=1}^N a_{ij} b_j(O_{t+1}) \beta_{t+1}(j),\qquad
&1 \leq j \leq N, \nonumber \\
&t = T-1, T-2, \dots, 1.
\label{eq:fw:back:loop}
\end{align}
